Validator/Expr/Grammar.lean
@@ -13,13 +13,14 @@ import Validator.Expr.Language
 --   𝑆 the start symbol of a regular hedge grammar is a regular expression comprising pairs of nonterminals and terminals (a regular expression over N × T)
 --   𝑃 a set of production rules of a regular hedge grammar are of the form X → r such that r is a regular expression over N × T.
 
-abbrev Ref μ := Fin μ -- non-terminal
+-- n = the number of non-terminals
+abbrev Ref (n: Nat) := Fin n -- non-terminal
 
-abbrev Rule (μ: Nat) (α: Type) (Φ: (α: Type) -> Type) :=
-  Regex (Φ α × Ref μ)
+abbrev Rule (n: Nat) (α: Type) (Φ: (α: Type) -> Type) :=
+  Regex (Φ α × Ref n)
 
-abbrev Rules (μ: Nat) (α: Type) (Φ: (α: Type) -> Type) (ν: Nat) :=
-  List.Vector (Rule μ α Φ) ν
+abbrev Rules (n: Nat) (α: Type) (Φ: (α: Type) -> Type) (l: Nat) :=
+  List.Vector (Rule n α Φ) l
 
 def hashVector [Hashable α] (xs: List.Vector α n): UInt64 :=
   hash xs.toList
@@ -27,18 +28,18 @@ def hashVector [Hashable α] (xs: List.Vector α n): UInt64 :=
 instance (α: Type) (n: Nat) [Hashable α] : Hashable (List.Vector α n) where
   hash := hashVector
 
-def hashRules {μ: Nat} {α: Type} {Φ: (α: Type) -> Type} {ν: Nat} [Hashable α] [Hashable (Φ α)] (xs: Rules μ α Φ ν): UInt64 :=
+def hashRules {n: Nat} {α: Type} {Φ: (α: Type) -> Type} {l: Nat} [Hashable α] [Hashable (Φ α)] (xs: Rules n α Φ l): UInt64 :=
   hash xs.toList
 
-instance (μ: Nat) (α: Type) (Φ: (α: Type) -> Type) (ν: Nat) [Hashable α] [Hashable (Φ α)] : Hashable (Rules μ α Φ ν) where
+instance (n: Nat) (α: Type) (Φ: (α: Type) -> Type) (l: Nat) [Hashable α] [Hashable (Φ α)] : Hashable (Rules n α Φ l) where
   hash := hashRules
 
-structure Grammar (μ: Nat) (α: Type) (Φ: (α: Type) -> Type) where
-  start: Rule μ α Φ
-  prods: Vector (Rule μ α Φ) μ
+structure Grammar (n: Nat) (α: Type) (Φ: (α: Type) -> Type) where
+  start: Rule n α Φ
+  prods: Vector (Rule n α Φ) n
 
-def Grammar.lookup {μ: Nat} {α: Type} {Φ: (α: Type) -> Type}
-  (g: Grammar μ α Φ) (ref: Fin μ): Rule μ α Φ :=
+def Grammar.lookup {n: Nat} {α: Type} {Φ: (α: Type) -> Type}
+  (g: Grammar n α Φ) (ref: Fin n): Rule n α Φ :=
   Vector.get g.prods ref
 
 def Grammar.singleton (x: Rule 0 α Φ): Grammar 0 α Φ  :=
@@ -90,7 +91,7 @@ theorem Rule.denote_decreasing {x: Hedge.Node α} {xs: Hedge α} (h: List.IsInfi
   simp +arith only at h
   omega
 
-def Rule.denote {α: Type} [BEq α] (g: Grammar μ α Pred) (r: Rule μ α Pred) (xs: Hedge α): Prop :=
+def Rule.denote {α: Type} [BEq α] (g: Grammar n α Pred) (r: Rule n α Pred) (xs: Hedge α): Prop :=
   Regex.denote_infix r xs (fun (pred, ref) xs' =>
     match xs' with
     | Subtype.mk [x] _hx =>
@@ -101,10 +102,10 @@ def Rule.denote {α: Type} [BEq α] (g: Grammar μ α Pred) (r: Rule μ α Pred)
   termination_by xs
   decreasing_by exact (Rule.denote_decreasing _hx)
 
-def Grammar.denote {α: Type} [BEq α] (g: Grammar μ α Pred) (xs: Hedge α): Prop :=
+def Grammar.denote {α: Type} [BEq α] (g: Grammar n α Pred) (xs: Hedge α): Prop :=
   Rule.denote g g.start xs
 
-theorem simp_denote_rule' {α: Type} [BEq α] (g: Grammar μ α Pred) (r: Rule μ α Pred) (xs: Hedge α):
+theorem simp_denote_rule' {α: Type} [BEq α] (g: Grammar n α Pred) (r: Rule n α Pred) (xs: Hedge α):
   (Regex.denote_infix r xs (fun (pred, ref) xs' =>
     match xs' with
     | Subtype.mk [x] _hx =>
@@ -132,7 +133,7 @@ theorem simp_denote_rule' {α: Type} [BEq α] (g: Grammar μ α Pred) (r: Rule �
     | nil =>
       simp
 
-theorem simp_denote_rule {α: Type} [BEq α] (g: Grammar μ α Pred) (r: Rule μ α Pred) (xs: Hedge α):
+theorem simp_denote_rule {α: Type} [BEq α] (g: Grammar n α Pred) (r: Rule n α Pred) (xs: Hedge α):
   Rule.denote g r xs =
   Regex.denote_infix r xs (fun (pred, ref) xs' =>
     ∃ label children, xs'.val = [Hedge.Node.mk label children] /\ Pred.eval pred label /\ Rule.denote g (g.lookup ref) children
@@ -155,22 +156,22 @@ theorem simp_denote_rule {α: Type} [BEq α] (g: Grammar μ α Pred) (r: Rule μ
     obtain ⟨label, children, hxs, h⟩ := h
     exists Hedge.Node.mk label children
 
-theorem Rule.denote_emptyset {α: Type} [BEq α] {g: Grammar μ α Pred}:
+theorem Rule.denote_emptyset {α: Type} [BEq α] {g: Grammar n α Pred}:
   Rule.denote g Regex.emptyset = Language.emptyset := by
   unfold Language.emptyset
   funext xs
   unfold Rule.denote
   simp [Regex.denote_infix_emptyset]
 
-theorem Rule.denote_emptystr {α: Type} [BEq α] {g: Grammar μ α Pred}:
+theorem Rule.denote_emptystr {α: Type} [BEq α] {g: Grammar n α Pred}:
   Rule.denote g Regex.emptystr = Language.emptystr := by
   unfold Language.emptystr
   funext xs
   unfold Rule.denote
   simp [Regex.denote_infix_emptystr]
 
-theorem denote_rule_symbol' {μ: Nat} {α: Type} [BEq α]
-  {g: Grammar μ α Pred} {pred: Pred α} {ref: Ref μ} {xs: Hedge α}:
+theorem denote_rule_symbol' {n: Nat} {α: Type} [BEq α]
+  {g: Grammar n α Pred} {pred: Pred α} {ref: Ref n} {xs: Hedge α}:
   Rule.denote g (Regex.symbol (pred, ref)) xs
   <-> Language.tree (Pred.eval pred) (Rule.denote g (g.lookup ref)) xs := by
   cases xs with
@@ -216,15 +217,15 @@ theorem denote_rule_symbol' {μ: Nat} {α: Type} [BEq α]
         rw [<- Rule.denote] at hg
         apply And.intro hp hg
 
-theorem Rule.denote_symbol {μ: Nat} {α: Type} [BEq α]
-  {g: Grammar μ α Pred} {pred: Pred α} {ref: Ref μ}:
+theorem Rule.denote_symbol {n: Nat} {α: Type} [BEq α]
+  {g: Grammar n α Pred} {pred: Pred α} {ref: Ref n}:
   Rule.denote g (Regex.symbol (pred, ref))
   = Language.tree (Pred.eval pred) (Rule.denote g (g.lookup ref)) := by
   funext xs
   rw [denote_rule_symbol']
 
-theorem Rule.denote_or {μ: Nat} {α: Type} [BEq α]
-  {g: Grammar μ α Pred} {p q: Rule μ α Pred}:
+theorem Rule.denote_or {n: Nat} {α: Type} [BEq α]
+  {g: Grammar n α Pred} {p q: Rule n α Pred}:
   Rule.denote g (Regex.or p q)
   = Language.or (Rule.denote g p) (Rule.denote g q) := by
   funext xs
@@ -232,8 +233,8 @@ theorem Rule.denote_or {μ: Nat} {α: Type} [BEq α]
   unfold Rule.denote
   simp [Regex.denote_infix_or]
 
-theorem Rule.denote_concat_n {μ: Nat} {α: Type} [BEq α]
-  {g: Grammar μ α Pred} {p q: Rule μ α Pred}:
+theorem Rule.denote_concat_n {n: Nat} {α: Type} [BEq α]
+  {g: Grammar n α Pred} {p q: Rule n α Pred}:
   Rule.denote g (Regex.concat p q)
   = Language.concat_n (Rule.denote g p) (Rule.denote g q) := by
   funext xs
@@ -277,16 +278,16 @@ theorem Rule.denote_concat_n {μ: Nat} {α: Type} [BEq α]
       | cons _ _ =>
         simp
 
-theorem Rule.denote_concat {μ: Nat} {α: Type} [BEq α]
-  {g: Grammar μ α Pred} {p q: Rule μ α Pred}:
+theorem Rule.denote_concat {n: Nat} {α: Type} [BEq α]
+  {g: Grammar n α Pred} {p q: Rule n α Pred}:
   Rule.denote g (Regex.concat p q)
   = Language.concat (Rule.denote g p) (Rule.denote g q) := by
   rw [Rule.denote_concat_n]
   funext xs
   rw [Language.concat_is_concat_n]
 
-theorem denote_rule_star_n' {μ: Nat} {α: Type} [BEq α]
-  {g: Grammar μ α Pred} {r: Rule μ α Pred} (xs: Hedge α):
+theorem denote_rule_star_n' {n: Nat} {α: Type} [BEq α]
+  {g: Grammar n α Pred} {r: Rule n α Pred} (xs: Hedge α):
   Rule.denote g (Regex.star r) xs
   <->
   Language.star_n (Rule.denote g r) xs := by
@@ -347,16 +348,16 @@ theorem denote_rule_star_n' {μ: Nat} {α: Type} [BEq α]
     obtain ⟨n, hn⟩ := n
     apply List.list_length_drop_lt_cons
 
-theorem Rule.denote_star_n {μ: Nat} {α: Type} [BEq α]
-  {g: Grammar μ α Pred} {r: Rule μ α Pred}:
+theorem Rule.denote_star_n {n: Nat} {α: Type} [BEq α]
+  {g: Grammar n α Pred} {r: Rule n α Pred}:
   Rule.denote g (Regex.star r)
   =
   Language.star_n (Rule.denote g r) := by
   funext xs
   rw [denote_rule_star_n']
 
-theorem Rule.denote_star {μ: Nat} {α: Type} [BEq α]
-  {g: Grammar μ α Pred} {r: Rule μ α Pred}:
+theorem Rule.denote_star {n: Nat} {α: Type} [BEq α]
+  {g: Grammar n α Pred} {r: Rule n α Pred}:
   Rule.denote g (Regex.star r)
   =
   Language.star (Rule.denote g r) := by
@@ -364,7 +365,7 @@ theorem Rule.denote_star {μ: Nat} {α: Type} [BEq α]
   rw [denote_rule_star_n']
   rw [Language.star_is_star_n]
 
-def Rule.denote_onlyif {α: Type} [BEq α] (condition: Prop) [dcond: Decidable condition] (g: Grammar μ α Pred) (x: Rule μ α Pred):
+def Rule.denote_onlyif {α: Type} [BEq α] (condition: Prop) [dcond: Decidable condition] (g: Grammar n α Pred) (x: Rule n α Pred):
   denote g (Regex.onlyif condition x) = Language.onlyif condition (denote g x) := by
   unfold Language.onlyif
   unfold Regex.onlyif
@@ -381,13 +382,13 @@ def Rule.denote_onlyif {α: Type} [BEq α] (condition: Prop) [dcond: Decidable c
     intro hc'
     contradiction
 
-def Rule.nullable (r: Rule μ α Φ): Bool :=
+def Rule.nullable (r: Rule n α Φ): Bool :=
   Regex.nullable r
 
-def Grammar.nullable (g: Grammar μ α Φ): Bool :=
+def Grammar.nullable (g: Grammar n α Φ): Bool :=
   Rule.nullable g.start
 
-theorem Rule.null_commutes {α: Type} [BEq α] (g: Grammar μ α Pred) (x: Rule μ α Pred):
+theorem Rule.null_commutes {α: Type} [BEq α] (g: Grammar n α Pred) (x: Rule n α Pred):
   ((Rule.nullable x) = true) = Language.null (denote g x) := by
   induction x with
   | emptyset =>
