Validator/Expr/IfExpr.lean
@@ -5,24 +5,24 @@ import Validator.Expr.Pred
 import Validator.Expr.Regex
 import Validator.Expr.Grammar
 
-inductive IfExpr μ α where
-  | mk (cnd: Pred α) (thn: Fin μ)
+inductive IfExpr n α where
+  | mk (cnd: Pred α) (thn: Fin n)
 
-abbrev IfExprs μ α ν := List.Vector (IfExpr μ α) ν
+abbrev IfExprs n α l := List.Vector (IfExpr n α) l
 
 namespace IfExpr
 
-def eval {α: Type} [DecidableEq α] (g: Grammar μ α Pred) (ifExpr: IfExpr μ α) (t: α): Rule μ α Pred :=
+def eval {α: Type} [DecidableEq α] (g: Grammar n α Pred) (ifExpr: IfExpr n α) (t: α): Rule n α Pred :=
   match ifExpr with
   | IfExpr.mk cnd thn =>
     if Pred.eval cnd t
     then g.lookup thn
     else Regex.emptyset
 
-def evals {α: Type} {μ: Nat} [DecidableEq α] (g: Grammar μ α Pred) (ifExprs: IfExprs μ α ν) (t: α): Rules μ α Pred ν :=
+def evals {α: Type} {n: Nat} [DecidableEq α] (g: Grammar n α Pred) (ifExprs: IfExprs n α l) (t: α): Rules n α Pred l :=
   List.Vector.map (fun x => eval g x t) ifExprs
 
-theorem evals_nil_is_nil {α: Type} {μ: Nat} [DecidableEq α] (g: Grammar μ α Pred) (a: α):
-  evals g (μ := μ) List.Vector.nil a = List.Vector.nil := by
+theorem evals_nil_is_nil {α: Type} {n: Nat} [DecidableEq α] (g: Grammar n α Pred) (a: α):
+  evals g (n := n) List.Vector.nil a = List.Vector.nil := by
   unfold evals
   simp
