Validator/Learning/Parser.lean
@@ -20,21 +20,21 @@ import Validator.Validator.Inst.TreeParserM
 
 namespace Parser
 
-def deriveEnter [DecidableEq α] [ValidateM m μ α] (g: Grammar μ α Pred) (xs: Rules μ α Pred ν): m (Rules μ α Pred (Symbol.nums xs)) := do
+def deriveEnter [DecidableEq α] [ValidateM m n α] (g: Grammar n α Pred) (xs: Rules n α Pred l): m (Rules n α Pred (Symbol.nums xs)) := do
   let enters <- Enter.DeriveEnter.deriveEnter xs
   let token <- Parser.token
   return IfExpr.evals g enters token
 
-def deriveLeaveM [DecidableEq α] [ValidateM m μ α] (xs: Rules μ α Pred ν) (cs: Rules μ α Pred (Symbol.nums xs)): m (Rules μ α Pred ν) :=
+def deriveLeaveM [DecidableEq α] [ValidateM m n α] (xs: Rules n α Pred l) (cs: Rules n α Pred (Symbol.nums xs)): m (Rules n α Pred l) :=
   Leave.DeriveLeaveM.deriveLeaveM xs (List.Vector.map Rule.nullable cs)
 
-def deriveValue [DecidableEq α] [ValidateM m μ α] (g: Grammar μ α Pred) (xs: Rules μ α Pred ν): m (Rules μ α Pred ν) := do
+def deriveValue [DecidableEq α] [ValidateM m n α] (g: Grammar n α Pred) (xs: Rules n α Pred l): m (Rules n α Pred l) := do
   deriveEnter g xs >>= deriveLeaveM xs
 
 -- TODO: Is it possible to have a Parser type that can be proved to be of the correct shape, and have not expection throwing
 -- for example: can you prove that your Parser will never return an Hint.leave after returning a Hint.field.
 -- This class can be called the LawfulParser.
-partial def derive [DecidableEq α] [ValidateM m μ α] (g: Grammar μ α Pred) (xs: Rules μ α Pred ν): m (Rules μ α Pred ν) := do
+partial def derive [DecidableEq α] [ValidateM m n α] (g: Grammar n α Pred) (xs: Rules n α Pred l): m (Rules n α Pred l) := do
   if List.all xs.toList Regex.unescapable then
     Parser.skip; return xs
   match <- Parser.next with
@@ -52,11 +52,11 @@ partial def derive [DecidableEq α] [ValidateM m μ α] (g: Grammar μ α Pred) 
   | Hint.leave => return xs -- never happens at the top
   | Hint.eof => return xs -- only happens at the top
 
-def validate {m} [DecidableEq α] [ValidateM m μ α] (g: Grammar μ α Pred) (x: Rule μ α Pred): m Bool := do
+def validate {m} [DecidableEq α] [ValidateM m n α] (g: Grammar n α Pred) (x: Rule n α Pred): m Bool := do
   let dxs <- derive g (List.Vector.cons x List.Vector.nil)
   return Rule.nullable dxs.head
 
-def run [DecidableEq α] (g: Grammar μ α Pred) (t: Hedge.Node α): Except String Bool :=
+def run [DecidableEq α] (g: Grammar n α Pred) (t: Hedge.Node α): Except String Bool :=
   TreeParserM.run' (validate g g.start) t
 
 -- Tests
@@ -69,7 +69,7 @@ open TokenTree (node)
   Except.ok false
 
 #guard run
-  (Grammar.mk (μ := 1)
+  (Grammar.mk (n := 1)
     (Regex.symbol (Pred.eq (Token.string "a"), 0))
     #v[Regex.emptystr]
   )
@@ -77,7 +77,7 @@ open TokenTree (node)
   Except.ok true
 
 #guard run
-  (Grammar.mk (μ := 1)
+  (Grammar.mk (n := 1)
     (Regex.symbol (Pred.eq (Token.string "a"), 0))
     #v[Regex.emptystr]
   )
@@ -85,7 +85,7 @@ open TokenTree (node)
   Except.ok false
 
 #guard run
-  (Grammar.mk (μ := 2)
+  (Grammar.mk (n := 2)
     (Regex.symbol (Pred.eq (Token.string "a"), 0))
     #v[
       (Regex.symbol (Pred.eq (Token.string "b"), 1))
@@ -96,7 +96,7 @@ open TokenTree (node)
   = Except.ok true
 
 #guard run
-  (Grammar.mk (μ := 2)
+  (Grammar.mk (n := 2)
     (Regex.symbol (Pred.eq (Token.string "a"), 0))
     #v[
       (Regex.concat
@@ -110,7 +110,7 @@ open TokenTree (node)
   Except.ok true
 
 #guard run
-  (Grammar.mk (μ := 3)
+  (Grammar.mk (n := 3)
     (Regex.symbol (Pred.eq (Token.string "a"), 0))
     #v[
       (Regex.concat
@@ -126,7 +126,7 @@ open TokenTree (node)
 
 -- try to engage skip using emptyset, since it is unescapable
 #guard run
-  (Grammar.mk (μ := 1)
+  (Grammar.mk (n := 1)
     (Regex.symbol (Pred.eq (Token.string "a"), 0))
     #v[Regex.emptyset]
   )
@@ -134,7 +134,7 @@ open TokenTree (node)
   = Except.ok false
 
 #guard run
-  (Grammar.mk (μ := 4)
+  (Grammar.mk (n := 4)
     (Regex.symbol (Pred.eq (Token.string "a"), 0))
     #v[
       (Regex.concat
@@ -150,7 +150,7 @@ open TokenTree (node)
   = Except.ok false
 
 #guard run
-  (Grammar.mk (μ := 2)
+  (Grammar.mk (n := 2)
     (Regex.symbol (Pred.eq (Token.string "a"), 0))
     #v[
       (Regex.concat
@@ -164,7 +164,7 @@ open TokenTree (node)
   Except.ok false
 
 #guard run
-  (Grammar.mk (μ := 3)
+  (Grammar.mk (n := 3)
     (Regex.symbol (Pred.eq (Token.string "a"), 0))
     #v[
       (Regex.concat
@@ -179,7 +179,7 @@ open TokenTree (node)
   = Except.ok false
 
 #guard run
-  (Grammar.mk (μ := 4)
+  (Grammar.mk (n := 4)
     (Regex.symbol (Pred.eq (Token.string "a"), 0))
     #v[
       (Regex.concat
