Validator/Validator/TestMem.lean
@@ -8,21 +8,21 @@ import Validator.Validator.Inst.TreeParserMemTestM
 
 namespace TestMem
 
-def validate {m} [DecidableEq α] [ValidateM m μ α] (g: Grammar μ α Pred) (x: Rule μ α Pred): m Bool :=
+def validate {m} [DecidableEq α] [ValidateM m n α] (g: Grammar n α Pred) (x: Rule n α Pred): m Bool :=
   Validate.validate g x
 
-def run [DecidableEq α] [Hashable α] (g: Grammar μ α Pred) (t: Hedge.Node α): Except String Bool :=
-  TreeParserMemM.run' (μ := μ) (validate g g.start) t
+def run [DecidableEq α] [Hashable α] (g: Grammar n α Pred) (t: Hedge.Node α): Except String Bool :=
+  TreeParserMemM.run' (n := n) (validate g g.start) t
 
 -- Tests
 
 def testCacheIsHitOnSecondRun
   [DecidableEq α] [Hashable α]
-  (g: Grammar μ α Pred) (t: Hedge.Node α): Except String Bool :=
-  match TreeParserMemM.run (μ := μ) (validate g g.start) t with
+  (g: Grammar n α Pred) (t: Hedge.Node α): Except String Bool :=
+  match TreeParserMemM.run (n := n) (validate g g.start) t with
   | EStateM.Result.error err _ => Except.error err
   | EStateM.Result.ok res1 state =>
-    match TreeParserMemTestM.runPopulatedMem (μ := μ) (validate g g.start) t state.enter state.leave with
+    match TreeParserMemTestM.runPopulatedMem (n := n) (validate g g.start) t state.enter state.leave with
     | EStateM.Result.error err _ => Except.error err
     | EStateM.Result.ok res2 _ =>
       if res1 ≠ res2
@@ -33,13 +33,13 @@ def testCacheIsHitOnSecondRun
 -- This tests that given an empty cache the test does actually fail.
 def testThatTestCacheBreaksWithEmptyCache
   [DecidableEq α] [Hashable α]
-  (g: Grammar μ α Pred) (t: Hedge.Node α): Except String Bool :=
-  TreeParserMemTestM.run' (μ := μ) (validate g g.start) t
+  (g: Grammar n α Pred) (t: Hedge.Node α): Except String Bool :=
+  TreeParserMemTestM.run' (n := n) (validate g g.start) t
 
 open TokenTree (node)
 
 #guard testCacheIsHitOnSecondRun
-  (Grammar.mk (μ := 1)
+  (Grammar.mk (n := 1)
     (Regex.symbol (Pred.eq (Token.string "a"), 0))
     #v[Regex.emptystr]
   )
@@ -47,7 +47,7 @@ open TokenTree (node)
   = Except.ok false
 
 #guard testCacheIsHitOnSecondRun
-  (Grammar.mk (μ := 1)
+  (Grammar.mk (n := 1)
     (Regex.symbol (Pred.eq (Token.string "a"), 0))
     #v[Regex.emptystr]
   )
@@ -55,7 +55,7 @@ open TokenTree (node)
   = Except.ok true
 
 #guard testThatTestCacheBreaksWithEmptyCache
-  (Grammar.mk (μ := 1)
+  (Grammar.mk (n := 1)
     (Regex.symbol (Pred.eq (Token.string "a"), 0))
     #v[Regex.emptystr]
   )
@@ -63,7 +63,7 @@ open TokenTree (node)
   = Except.error "test cache miss"
 
 #guard testCacheIsHitOnSecondRun
-  (Grammar.mk (μ := 1)
+  (Grammar.mk (n := 1)
     (Regex.symbol (Pred.eq (Token.string "a"), 0))
     #v[Regex.emptystr]
   )
@@ -71,7 +71,7 @@ open TokenTree (node)
   = Except.ok false
 
 #guard testCacheIsHitOnSecondRun
-  (Grammar.mk (μ := 2)
+  (Grammar.mk (n := 2)
     (Regex.symbol (Pred.eq (Token.string "a"), 0))
     #v[
       (Regex.symbol (Pred.eq (Token.string "b"), 1))
@@ -82,7 +82,7 @@ open TokenTree (node)
   = Except.ok true
 
 #guard testCacheIsHitOnSecondRun
-  (Grammar.mk (μ := 2)
+  (Grammar.mk (n := 2)
     (Regex.symbol (Pred.eq (Token.string "a"), 0))
     #v[
       (Regex.concat
@@ -96,7 +96,7 @@ open TokenTree (node)
   = Except.ok true
 
 #guard testCacheIsHitOnSecondRun
-  (Grammar.mk (μ := 3)
+  (Grammar.mk (n := 3)
     (Regex.symbol (Pred.eq (Token.string "a"), 0))
     #v[
       (Regex.concat
@@ -112,7 +112,7 @@ open TokenTree (node)
 
 -- try to engage skip using emptyset, since it is unescapable
 #guard testCacheIsHitOnSecondRun
-  (Grammar.mk (μ := 1)
+  (Grammar.mk (n := 1)
     (Regex.symbol (Pred.eq (Token.string "a"), 0))
     #v[Regex.emptyset]
   )
@@ -120,7 +120,7 @@ open TokenTree (node)
   = Except.ok false
 
 #guard testCacheIsHitOnSecondRun
-  (Grammar.mk (μ := 4)
+  (Grammar.mk (n := 4)
     (Regex.symbol (Pred.eq (Token.string "a"), 0))
     #v[
       (Regex.concat
@@ -136,7 +136,7 @@ open TokenTree (node)
   = Except.ok false
 
 #guard testCacheIsHitOnSecondRun
-  (Grammar.mk (μ := 2)
+  (Grammar.mk (n := 2)
     (Regex.symbol (Pred.eq (Token.string "a"), 0))
     #v[
       (Regex.concat
@@ -150,7 +150,7 @@ open TokenTree (node)
   Except.ok false
 
 #guard testCacheIsHitOnSecondRun
-  (Grammar.mk (μ := 3)
+  (Grammar.mk (n := 3)
     (Regex.symbol (Pred.eq (Token.string "a"), 0))
     #v[
       (Regex.concat
@@ -165,7 +165,7 @@ open TokenTree (node)
   = Except.ok false
 
 #guard testCacheIsHitOnSecondRun
-  (Grammar.mk (μ := 4)
+  (Grammar.mk (n := 4)
     (Regex.symbol (Pred.eq (Token.string "a"), 0))
     #v[
       (Regex.concat
